theory/Interpreter.thy
@@ -839,14 +839,14 @@ value "bpf_interp_test
 
 value "loadv M8 (u8_list_to_mem (int_to_u8_list [0x01, 0x02, 0x03, 0x04, 0x05, 0x06, 0x07, 0x08, 0x09])) 2" *)
 
-(*
+
 value "loadv M16 (u8_list_to_mem (int_to_u8_list [0x11, 0x22, 0x33])) 1"
 (**r return 0x3322 = 13090 *)
 value "(u16_of_u8_list (rev (u8_list_of_u16 (ucast (0x3322::u64)))))"
 (**r return 0x2233 = 8755 *)
 value "case storev M16 init_mem 0 (Vshort 0x1122) of None \<Rightarrow> None | Some m \<Rightarrow> loadv M16 m 0"
 (**r return 0x1122 =4386 *)
-*)
+
 
 
 lemma "((ucast ((ucast (i::i32))::u64)) :: u32) = ((ucast (i::i32))::u32)"
